\documentclass{article}  %Need this.

\usepackage{amsmath,amsthm,amssymb}

%\usepackage[margin=1in]{geometry}


\newtheorem*{thm}{Theorem}
\newtheorem*{cnj}{Conjecture}
\newtheorem*{lem}{Lemma}
\newtheorem*{cor}{Corollary}
\newtheorem*{prop}{Proposition}

\newcommand{\N}{\mathbb{N}}
\newcommand{\Z}{\mathbb{Z}}
\newcommand{\R}{\mathbb{R}}





\title{Reproducing a \LaTeX Document}
\author{Put your name here}
\date{}


\begin{document}
\maketitle

\begin{thm}
If $x$ and $y$ are odd integers then $x+y$ is an even integer.
\end{thm}

\begin{proof}
We assume that $x$ and $y$ are odd integers and will prove that $x+y$ is an even integer. Since $x$ and $y$ are odd, there exist integers $m$ and $n$ such that $x=2m+1$ and $y=2n+1$.  By substitution and algebra we obtain
\begin{align*}
x+y &= 2m+1 + 2n + 1\\
&= 2m+2n+2\\
&=2(m+n+1).
\end{align*}
Define $q=m+n+1$.  Since $m$ and $n$ are integers and the integers are closed under addition, we conclude that $q$ is an integer. Since $x+y=2q$ for the integer $q$ we conclude that $x+y$ is an even integer.
\end{proof}


\vspace{.15in}

\section*{Challenge Typing}


Suppose that $f:(-1,1)\to \R$ and $f$ is differentiable at $0$. Let sequences $(\alpha_n)_{n\geq1}$ and $(\beta_n)_{n\geq1}$ satisify $-1<\alpha_n<\beta_n<1$ for all $n\geq 1$ and $\displaystyle{\lim_{n\to\infty}} \alpha_n = \displaystyle{\lim_{n\to\infty}} \beta_n = 0$. Set 
	
		$$\lambda_n = \frac{f(\beta_n) -f(\alpha_n)}{\beta_n-\alpha_n} . $$



\end{document}